Start adding fullStorages to the domain
For account creation we want to be able to reserve the whole storage
(which should be completely empty before an account is created) without
listing every key in the storageKeys part of the domain.

spec/vfmExecutionScript.sml
@@ -119,7 +119,7 @@ Datatype:
   | InvalidContractPrefix
   | Reverted
   (* semantic invariants/assumptions (not EVM exceptions) *)
-  | OutsideDomain (address + storage_key)
+  | OutsideDomain (address + storage_key + address)
   | Unimplemented
   | Impossible
 End
@@ -433,7 +433,13 @@ Definition access_slot_def:
       return
         (if fIN x storageKeys then warm_access_cost else cold_sload_cost)
         (s with rollback := newRollback)
-  else fail (OutsideDomain (INR x)) s
+  else fail (OutsideDomain (INR (INL x))) s
+End
+
+Definition ensure_storage_in_domain_def:
+  ensure_storage_in_domain a s =
+    assert (fIN a s.msdomain.fullStorages)
+           (OutsideDomain (INR (INR a))) s
 End
 
 Definition zero_warm_def:
@@ -1036,6 +1042,7 @@ Definition step_create_def:
     assert_not_static;
     set_return_data [];
     sucDepth <- get_num_contexts;
+    ensure_storage_in_domain address;
     toCreate <<- lookup_account address accounts;
     if sender.balance < value ∨
        SUC nonce ≥ 2 ** 64 ∨
